ExpressionsTutorial: PHOAS without yet taking advantage of sharing

Kami/Ex/ExpressionsTutorial.v
@@ -1,45 +1,32 @@
-Require Import Arith NatLib Ring ArithRing Omega.
+Require Import Arith NatLib Ring ArithRing Omega Vector.
 Require Import Kami.
 
 
 (** * Warm-up: words (bitvectors) *)
 
 Definition B := word 8.
-Definition multibyte := list B.
+Definition multibyte := Vector.t B.
 
-Fixpoint mbToNat (mb : multibyte) : nat :=
+Fixpoint mbToNat {len} (mb : multibyte len) : nat :=
   match mb with
-  | nil => 0
-  | b :: mb' => wordToNat b + mbToNat mb' * 256
+  | Vector.nil _ => 0
+  | Vector.cons _ b _ mb' => wordToNat b + mbToNat mb' * 256
   end.
 
-Fixpoint applyCarry (carry : word 1) (mb : multibyte) : multibyte :=
-  match mb with
-  | nil => combine carry (wzero 7) :: nil
-  | b :: mb' =>
+Fixpoint mbAdd' {len} (carry : word 1) : multibyte len -> multibyte len -> multibyte (S len) :=
+  match len with
+  | O => fun _ _ => Vector.cons _ (combine carry (wzero 7)) _ (Vector.nil _)
+  | S len' => fun mb1 mb2 =>
     let carry_9 := combine carry (wzero 8) in
-    let b_9 := combine b (wzero 1) in
-    let sum_9 := carry_9 ^+ b_9 in
-    let sum_8 := split1 8 1 sum_9 in
-    let carry' := split2 8 1 sum_9 in
-    sum_8 :: applyCarry carry' mb'
-  end.
-
-Fixpoint mbAdd' (carry : word 1) (mb1 mb2 : multibyte) : multibyte :=
-  match mb1, mb2 with
-  | nil, _ => applyCarry carry mb2
-  | _, nil => applyCarry carry mb1
-  | b1 :: mb1', b2 :: mb2' =>
-    let carry_9 := combine carry (wzero 8) in
-    let b1_9 := combine b1 (wzero 1) in
-    let b2_9 := combine b2 (wzero 1) in
+    let b1_9 := combine (Vector.hd mb1) (wzero 1) in
+    let b2_9 := combine (Vector.hd mb2) (wzero 1) in
     let sum_9 := carry_9 ^+ b1_9 ^+ b2_9 in
     let sum_8 := split1 8 1 sum_9 in
     let carry' := split2 8 1 sum_9 in
-    sum_8 :: mbAdd' carry' mb1' mb2'
+    Vector.cons _ sum_8 _ (mbAdd' carry' (Vector.tl mb1) (Vector.tl mb2))
   end.
 
-Definition mbAdd := mbAdd' (wzero 1).
+Definition mbAdd {len} := mbAdd' (len := len) (wzero 1).
 
 Lemma split_plus : forall b a (w : word (a + b)),
     wordToNat (split1 a b w) + wordToNat (split2 a b w) * pow2 a = wordToNat w.
@@ -91,56 +78,25 @@ Qed.
 
 Opaque wordToNat natToWord split1 split2 combine.
 
-Lemma applyCarry_ok : forall mb carry,
-    mbToNat (applyCarry carry mb)
-    = wordToNat carry + mbToNat mb.
+Lemma shatter_vector : forall {A n} (v : Vector.t A n),
+    match n return Vector.t A n -> Prop with
+    | O => fun v => v = Vector.nil _
+    | S n' => fun v => exists h t, v = Vector.cons _ h _ t
+    end v.
 Proof.
-  induction mb; simpl; intuition.
-
-  {
-    pose proof (shatter_word_S carry).
-    destruct H as [b [c Heq]]; subst.
-    simpl.
-    pose proof (shatter_word_0 c); subst.
-    destruct b; simpl.
-    reflexivity.
-    reflexivity.
-  }
-
-  {
-    rewrite IHmb.
-    ring_simplify.
-    pose proof (split_plus 1 8 (combine carry (wzero 8) ^+ combine a (wzero 1))).
-    change (pow2 8) with 256 in *.
-    pose proof (pad_with_zero _ carry 8).
-    pose proof (pad_with_zero _ a 1).
-    simpl in H, H0, H1.
-    rewrite wplus_nowrap in H.
-
-    {
-      rewrite H0, H1 in H.
-      rewrite <- (plus_assoc _ _ (wordToNat a)).
-      rewrite <- H.
-      ring.
-    }
-
-    {
-      rewrite H0, H1.
-      pose proof (wordToNat_bound carry).
-      pose proof (wordToNat_bound a).
-      simpl in *.
-      omega.
-    }
-  }
+  destruct v; eauto.
 Qed.
 
-Lemma mbAdd'_ok : forall mb1 mb2 carry,
+Lemma mbAdd'_ok : forall len (mb1 mb2 : multibyte len) carry,
     mbToNat (mbAdd' carry mb1 mb2)
     = wordToNat carry + mbToNat mb1 + mbToNat mb2.
 Proof.
-  induction mb1; destruct mb2; simpl; intuition.
+  induction len; simpl; intuition.
 
   {
+    pose proof (shatter_vector mb1).
+    pose proof (shatter_vector mb2).
+    simpl in *; subst; simpl.
     pose proof (shatter_word_S carry).
     destruct H as [b [c Heq]]; subst.
     simpl.
@@ -148,62 +104,15 @@ Proof.
     destruct b; simpl.
     reflexivity.
     reflexivity.
-  }    
+  }
   
   {
-    rewrite applyCarry_ok.
-    ring_simplify.
-    pose proof (split_plus 1 8 (combine carry (wzero 8) ^+ combine b (wzero 1))).
-    change (pow2 8) with 256 in *.
-    pose proof (pad_with_zero _ carry 8).
-    pose proof (pad_with_zero _ b 1).
-    simpl in H, H0, H1.
-    rewrite wplus_nowrap in H.
-
-    {
-      rewrite H0, H1 in H.
-      rewrite <- (plus_assoc _ _ (wordToNat b)).
-      rewrite <- H.
-      ring.
-    }
-
-    {
-      rewrite H0, H1.
-      pose proof (wordToNat_bound carry).
-      pose proof (wordToNat_bound b).
-      simpl in *.
-      omega.
-    }
-  }
-
-  {
-    rewrite applyCarry_ok.
-    ring_simplify.
-    pose proof (split_plus 1 8 (combine carry (wzero 8) ^+ combine a (wzero 1))).
-    change (pow2 8) with 256 in *.
-    pose proof (pad_with_zero _ carry 8).
-    pose proof (pad_with_zero _ a 1).
-    simpl in H, H0, H1.
-    rewrite wplus_nowrap in H.
-
-    {
-      rewrite H0, H1 in H.
-      rewrite <- (plus_assoc _ _ (wordToNat a)).
-      rewrite <- H.
-      ring.
-    }
-
-    {
-      rewrite H0, H1.
-      pose proof (wordToNat_bound carry).
-      pose proof (wordToNat_bound a).
-      simpl in *.
-      omega.
-    }
-  }
-
-  {
-    rewrite IHmb1.
+    pose proof (shatter_vector mb1).
+    pose proof (shatter_vector mb2).
+    simpl in *; subst; simpl.
+    destruct H as [a [mb1' ?]]; subst.
+    destruct H0 as [b [mb2' ?]]; subst.
+    rewrite IHlen; simpl.
     ring_simplify.
     pose proof (split_plus 1 8 (combine carry (wzero 8) ^+ combine a (wzero 1) ^+ combine b (wzero 1))).
     change (pow2 8) with 256 in *.
@@ -215,8 +124,8 @@ Proof.
 
     {
       rewrite H0, H1, H2 in H.
-      replace (256 * mbToNat mb1 + 256 * mbToNat mb2 + # (carry) + # (a) + # (b))
-              with (256 * mbToNat mb1 + 256 * mbToNat mb2 + (# (carry) + # (a) + # (b))) by omega.
+      replace (256 * mbToNat mb1' + 256 * mbToNat mb2' + # (carry) + # (a) + # (b))
+              with (256 * mbToNat mb1' + 256 * mbToNat mb2' + (# (carry) + # (a) + # (b))) by omega.
       rewrite <- H.
       ring.
     }
@@ -252,7 +161,7 @@ Proof.
   }
 Qed.
 
-Theorem mbAdd_ok : forall mb1 mb2,
+Theorem mbAdd_ok : forall len (mb1 mb2 : multibyte len),
     mbToNat (mbAdd mb1 mb2)
     = mbToNat mb1 + mbToNat mb2.
 Proof.
@@ -264,98 +173,237 @@ Qed.
 
 (** * Introducing a deeply embedded language *)
 
-Inductive expr : nat -> Type :=
-| Const : forall {n}, word n -> expr n
-| Combine : forall {n1 n2}, expr n1 -> expr n2 -> expr (n1 + n2)
-| Split1 : forall {n1 n2}, expr (n1 + n2) -> expr n1
-| Split2 : forall {n1 n2}, expr (n1 + n2) -> expr n2
-| Add : forall {n}, expr n -> expr n -> expr n.
+Notation "[ x1 ; .. ; xN ]" := (Vector.cons _ x1 _ (.. (Vector.cons _ xN _ (Vector.nil _)) ..)).
 
-Definition Multibyte := list (expr 8).
-
-Fixpoint ApplyCarry (carry : expr 1) (mb : Multibyte) : Multibyte :=
-  match mb with
-  | nil =>
-    Combine carry (Const (wzero 7)) :: nil
-  | b :: mb' =>
-    let carry_9 := Combine carry (Const (wzero 8)) in
-    let b_9 := Combine b (Const (wzero 1)) in
-    let sum_9 := Add carry_9 b_9 in
-    let sum_8 := Split1 (n1 := 8) (n2 := 1) sum_9 in
-    let carry' := Split2 (n1 := 8) (n2 := 1) sum_9 in
-    sum_8 :: ApplyCarry carry' mb'
-  end.
-
-Fixpoint MbAdd' (carry : expr 1) (mb1 mb2 : Multibyte) : Multibyte :=
-  match mb1, mb2 with
-  | nil, _ => ApplyCarry carry mb2
-  | _, nil => ApplyCarry carry mb1
-  | b1 :: mb1', b2 :: mb2' =>
-    let carry_9 := Combine carry (Const (wzero 8)) in
-    let b1_9 := Combine b1 (Const (wzero 1)) in
-    let b2_9 := Combine b2 (Const (wzero 1)) in
-    let sum_9 := Add (Add carry_9 b1_9) b2_9 in
-    let sum_8 := Split1 (n1 := 8) (n2 := 1) sum_9 in
-    let carry' := Split2 (n1 := 8) (n2 := 1) sum_9 in
-    sum_8 :: MbAdd' carry' mb1' mb2'
-  end.
-
-Definition MbAdd := MbAdd' (Const (wzero 1)).
-
-(** ** Semantics *)
-
-Fixpoint interp {n} (e : expr n) : word n :=
-  match e with
-  | Const k => k
-  | Combine e1 e2 => combine (interp e1) (interp e2)
-  | Split1 e1 => split1 _ _ (interp e1)
-  | Split2 e2 => split2 _ _ (interp e2)
-  | Add e1 e2 => interp e1 ^+ interp e2
-  end.
-
-Lemma ApplyCarry_encoded_properly : forall mb carry,
-    map interp (ApplyCarry carry mb) = applyCarry (interp carry) (map interp mb).
-Proof.
-  induction mb; simpl; intuition.
-
-  rewrite IHmb.
-  reflexivity.
-Qed.
-
-Lemma MbAdd'_encoded_properly : forall mb1 mb2 carry,
-    map interp (MbAdd' carry mb1 mb2) = mbAdd' (interp carry) (map interp mb1) (map interp mb2).
-Proof.
-  induction mb1; destruct mb2; simpl; intuition.
-
-  {
-    rewrite ApplyCarry_encoded_properly.
-    reflexivity.
-  }
-
-  {
-    rewrite ApplyCarry_encoded_properly.
-    reflexivity.
-  }
-
-  {
-    rewrite IHmb1.
-    reflexivity.
-  }
-Qed.
-
-Lemma MbAdd_encoded_properly : forall mb1 mb2,
-    map interp (MbAdd mb1 mb2) = mbAdd (map interp mb1) (map interp mb2).
-Proof.
-  unfold MbAdd, mbAdd; intros.
-  rewrite MbAdd'_encoded_properly.
-  reflexivity.
-Qed.
-
-Theorem MbAdd_ok : forall mb1 mb2,
-    mbToNat (map interp (MbAdd mb1 mb2))
-    = mbToNat (map interp mb1) + mbToNat (map interp mb2).
+Lemma hd_map : forall {A B len} (f : A -> B) (v : Vector.t A (S len)),
+    Vector.hd (Vector.map f v) = f (Vector.hd v).
 Proof.
   intros.
-  rewrite MbAdd_encoded_properly.
-  apply mbAdd_ok.
+  pose proof (shatter_vector v); simpl in *.
+  destruct H as [a [v' ?]]; subst.
+  reflexivity.
 Qed.
+
+Lemma tl_map : forall {A B len} (f : A -> B) (v : Vector.t A (S len)),
+    Vector.tl (Vector.map f v) = Vector.map f (Vector.tl v).
+Proof.
+  intros.
+  pose proof (shatter_vector v); simpl in *.
+  destruct H as [a [v' ?]]; subst.
+  reflexivity.
+Qed.
+
+Module DeeplyEmbedded.
+  Inductive expr : nat -> Type :=
+  | Const : forall {n}, word n -> expr n
+  | Combine : forall {n1 n2}, expr n1 -> expr n2 -> expr (n1 + n2)
+  | Split1 : forall {n1 n2}, expr (n1 + n2) -> expr n1
+  | Split2 : forall {n1 n2}, expr (n1 + n2) -> expr n2
+  | Add : forall {n}, expr n -> expr n -> expr n.
+
+  Definition Multibyte := Vector.t (expr 8).
+
+  Fixpoint MbAdd' {len} (carry : expr 1) : Multibyte len -> Multibyte len -> Multibyte (S len) :=
+    match len with
+    | 0 => fun _ _ => Vector.cons _ (Combine carry (Const (wzero 7))) _ (Vector.nil _)
+    | S len' => fun mb1 mb2 =>
+      let carry_9 := Combine carry (Const (wzero 8)) in
+      let b1_9 := Combine (Vector.hd mb1) (Const (wzero 1)) in
+      let b2_9 := Combine (Vector.hd mb2) (Const (wzero 1)) in
+      let sum_9 := Add (Add carry_9 b1_9) b2_9 in
+      let sum_8 := Split1 (n1 := 8) (n2 := 1) sum_9 in
+      let carry' := Split2 (n1 := 8) (n2 := 1) sum_9 in
+      Vector.cons _ sum_8 _ (MbAdd' carry' (Vector.tl mb1) (Vector.tl mb2))
+    end.
+
+  Definition MbAdd {len} := MbAdd' (len := len) (Const (wzero 1)).
+
+  (** ** Semantics *)
+
+  Fixpoint interp {n} (e : expr n) : word n :=
+    match e with
+    | Const k => k
+    | Combine e1 e2 => combine (interp e1) (interp e2)
+    | Split1 e1 => split1 _ _ (interp e1)
+    | Split2 e2 => split2 _ _ (interp e2)
+    | Add e1 e2 => interp e1 ^+ interp e2
+    end.
+
+  Lemma MbAdd'_encoded_properly : forall len (mb1 mb2 : Multibyte len) carry,
+      Vector.map interp (MbAdd' carry mb1 mb2)
+      = mbAdd' (interp carry) (Vector.map interp mb1) (Vector.map interp mb2).
+  Proof.
+    induction len; simpl; intuition.
+
+    rewrite IHlen.
+    simpl.
+    repeat rewrite hd_map, tl_map.
+    reflexivity.
+  Qed.
+
+  Lemma MbAdd_encoded_properly : forall len (mb1 mb2 : Multibyte len),
+      Vector.map interp (MbAdd mb1 mb2)
+      = mbAdd (Vector.map interp mb1) (Vector.map interp mb2).
+  Proof.
+    unfold MbAdd, mbAdd; intros.
+    rewrite MbAdd'_encoded_properly.
+    reflexivity.
+  Qed.
+
+  Theorem MbAdd_ok : forall len (mb1 mb2 : Multibyte len),
+      mbToNat (Vector.map interp (MbAdd mb1 mb2))
+      = mbToNat (Vector.map interp mb1) + mbToNat (Vector.map interp mb2).
+  Proof.
+    intros.
+    rewrite MbAdd_encoded_properly.
+    apply mbAdd_ok.
+  Qed.
+
+  (** ** Trouble in paradise *)
+
+  Definition add2 a1 a2 b1 b2 := MbAdd [a1; a2] [b1; b2].
+  Compute add2.
+
+  Definition add3 a1 a2 a3 b1 b2 b3 := MbAdd [a1; a2; a3] [b1; b2; b3].
+  Compute add3.
+End DeeplyEmbedded.
+
+
+(** * Parametric Higher-Order Abstract Syntax *)
+
+Module Phoas.
+  Section var.
+    Context {var : nat -> Type}.
+
+    Inductive expr : nat -> Type :=
+    | Const : forall {n}, word n -> expr n
+    | Combine : forall {n1 n2}, expr n1 -> expr n2 -> expr (n1 + n2)
+    | Split1 : forall {n1 n2}, expr (n1 + n2) -> expr n1
+    | Split2 : forall {n1 n2}, expr (n1 + n2) -> expr n2
+    | Add : forall {n}, expr n -> expr n -> expr n
+
+    | Var : forall {n}, var n -> expr n
+    | LetIn : forall {n1 n2}, expr n1 -> (var n1 -> expr n2) -> expr n2.
+  End var.
+
+  Arguments expr : clear implicits.
+
+  Definition Expr n := forall var, expr var n.
+
+  Section var'.
+    Context {var : nat -> Type}.
+
+    Definition Multibyte' := Vector.t (expr var 8).
+
+    Fixpoint MbAdd' {len} (carry : expr var 1) : Multibyte' len -> Multibyte' len -> expr var (len * 8 + 8) :=
+      match len with
+      | 0 => fun _ _ => Combine carry (Const (wzero 7))
+      | S len' => fun mb1 mb2 =>
+        let carry_9 := Combine carry (Const (wzero 8)) in
+        let b1_9 := Combine (Vector.hd mb1) (Const (wzero 1)) in
+        let b2_9 := Combine (Vector.hd mb2) (Const (wzero 1)) in
+        let sum_9 := Add (Add carry_9 b1_9) b2_9 in
+        let sum_8 := Split1 (n1 := 8) (n2 := 1) sum_9 in
+        let carry' := Split2 (n1 := 8) (n2 := 1) sum_9 in
+        Combine sum_8 (MbAdd' carry' (Vector.tl mb1) (Vector.tl mb2))
+      end.
+  End var'.
+
+  Arguments Multibyte' : clear implicits.  
+
+  Definition Multibyte len := forall var, Multibyte' var len.
+  Definition MbAdd {len} (mb1 mb2 : Multibyte len) : Expr (len * 8 + 8) := 
+    fun var => MbAdd' (Const (wzero 1)) (mb1 var) (mb2 var).
+
+  (** ** Semantics *)
+
+  Fixpoint interp {n} (e : expr word n) : word n :=
+    match e with
+    | Const k => k
+    | Combine e1 e2 => combine (interp e1) (interp e2)
+    | Split1 e1 => split1 _ _ (interp e1)
+    | Split2 e2 => split2 _ _ (interp e2)
+    | Add e1 e2 => interp e1 ^+ interp e2
+
+    | Var k => k
+    | LetIn e1 e2 => interp (e2 (interp e1))
+    end.
+
+  Definition Interp {n} (E : Expr n) : word n := interp (E word).
+
+  Fixpoint flatten {len} : multibyte (S len) -> word (len * 8 + 8) :=
+    match len with
+    | O => fun w => Vector.hd w
+    | S len' => fun w => combine (Vector.hd w) (flatten (Vector.tl w))
+    end.
+
+  Lemma MbAdd'_encoded_properly : forall len (mb1 mb2 : Multibyte' word len) carry,
+      interp (MbAdd' carry mb1 mb2)
+      = flatten (mbAdd' (interp carry) (Vector.map interp mb1) (Vector.map interp mb2)).
+  Proof.
+    induction len; simpl; intuition.
+
+    rewrite IHlen.
+    simpl.
+    repeat rewrite hd_map, tl_map.
+    reflexivity.
+  Qed.
+
+  Lemma MbAdd_encoded_properly : forall len (mb1 mb2 : Multibyte len),
+      Interp (MbAdd mb1 mb2)
+      = flatten (mbAdd (Vector.map interp (mb1 word)) (Vector.map interp (mb2 word))).
+  Proof.
+    unfold MbAdd, mbAdd, Interp; intros.
+    rewrite MbAdd'_encoded_properly.
+    reflexivity.
+  Qed.
+
+  Opaque wordToNat split1 split2 combine pow2.
+
+  Lemma flatten_ok : forall len (mb : multibyte (S len)),
+      wordToNat (flatten mb) = mbToNat mb.
+  Proof.
+    induction len; simpl; intuition.
+
+    {
+      pose proof (shatter_vector mb); simpl in *.
+      destruct H as [a [mb']]; subst.
+      simpl.
+      pose proof (shatter_vector mb'); simpl in *; subst.
+      simpl.
+      omega.
+    }
+
+    {
+      pose proof (wordToNat_combine (Vector.hd mb) (flatten (Vector.tl mb))).
+      simpl in *.
+      rewrite H.
+      pose proof (shatter_vector mb); simpl in *.      
+      destruct H0 as [a [mb']]; subst.
+      simpl.
+      rewrite IHlen.
+      change (pow2 8) with 256.
+      omega.
+    }
+  Qed.
+
+  Theorem MbAdd_ok : forall len (mb1 mb2 : Multibyte len),
+      wordToNat (Interp (MbAdd mb1 mb2))
+      = mbToNat (Vector.map interp (mb1 word)) + mbToNat (Vector.map interp (mb2 word)).
+  Proof.
+    intros.
+    rewrite MbAdd_encoded_properly.
+    rewrite flatten_ok.
+    apply mbAdd_ok.
+  Qed.
+
+  (** ** Less trouble in paradise *)
+
+  Definition add2 {var : nat -> Type} (a1 a2 b1 b2 : var 8) :=
+    MbAdd' (Const (wzero 1)) [Var a1; Var a2] [Var b1; Var b2].
+  Compute add2.
+
+  Definition add3 {var : nat -> Type} (a1 a2 a3 b1 b2 b3 : var 8) :=
+    MbAdd' (Const (wzero 1)) [Var a1; Var a2; Var a3] [Var b1; Var b2; Var b3].
+  Compute add3.
+End Phoas.
